Pm4Lean/Models/Petri/WFNet/WOFLAN/Boundedness/SelfCover/Definitions.lean
@@ -1,0 +1,2 @@
+import Pm4Lean.Models.Petri.WFNet.WOFLAN.Boundedness.SelfCover.Definitions.Covers
+import Pm4Lean.Models.Petri.WFNet.WOFLAN.Boundedness.SelfCover.Definitions.Extraction
